src/tls/AEAD_GCM.fst
@@ -2,13 +2,11 @@ module AEAD_GCM
 // AEAD-GCM mode for the TLS record layer, as specified in RFC 5288.
 // We support both AES_128_GCM and AES_256_GCM, differing only in their key sizes
 
-open FStar.Heap
-open FStar.HyperHeap
-open FStar.HyperStack
 open FStar.Seq
 open Platform.Bytes
 open CoreCrypto
 
+open Mem
 open TLSConstants
 open TLSInfo
 open LHAEPlain
@@ -73,7 +71,7 @@ let ctr (#l:rgn) (#r:rgn) (#i:id) (#log:log_ref l i) (c:ctr_ref r i log)
 // kept concrete for log and counter, but the key and iv should be private.
 noeq type state (i:id) (rw:rw) =
   | State: #region: rgn
-         -> #log_region: rgn{if rw = Writer then region = log_region else HyperHeap.disjoint region log_region}
+         -> #log_region: rgn{if rw = Writer then region = log_region else disjoint region log_region}
          -> aead: AEAD.state i rw
          -> log: log_ref log_region i // ghost subject to cryptographic assumption
          -> counter: ctr_ref region i log // types are sufficient to anti-alias log and counter
@@ -97,11 +95,11 @@ type matching (#i:id) (r:reader i) (w:writer i) =
 let genPost (#i:id) parent h0 (w:writer i) h1 =
   modifies Set.empty h0 h1 /\
   extends w.region parent /\
-  stronger_fresh_region w.region h0 h1 /\
+  fresh_region w.region h0 h1 /\
   disjoint w.region (AEAD.log_region w.aead) /\
   color w.region = color parent /\
   extends (AEAD.region w.aead) parent /\
-  stronger_fresh_region (AEAD.region w.aead) h0 h1 /\
+  fresh_region (AEAD.region w.aead) h0 h1 /\
   color (AEAD.region w.aead) = color parent /\
   AEAD.empty_log w.aead h1 /\
   (authId i ==> (m_contains (ilog w.log) h1 /\ m_sel h1 (ilog w.log) == createEmpty)) /\
@@ -131,21 +129,21 @@ let gen parent i =
 
 val genReader: parent:rgn -> #i:id -> w:writer i -> ST (reader i)
   (requires (fun h0 ->
-    HyperHeap.disjoint parent w.region /\
-    HyperHeap.disjoint parent (AEAD.region w.aead)))
+    disjoint parent w.region /\
+    disjoint parent (AEAD.region w.aead)))
   (ensures  (fun h0 (r:reader i) h1 ->
     modifies Set.empty h0 h1 /\
     r.log_region = w.region /\
     extends r.region parent /\
     color r.region = color parent /\
-    stronger_fresh_region r.region h0 h1 /\
+    fresh_region r.region h0 h1 /\
     eq2 #(log_ref w.log_region i) w.log r.log /\
     m_contains (ctr r.counter) h1 /\
     m_sel h1 (ctr r.counter) === 0))
 let genReader parent #i w =
   let reader_r = new_region parent in
   let wr : rgn = w.region in
-  assert(HyperHeap.disjoint wr reader_r);
+  assert(disjoint wr reader_r);
   let raead = AEAD.genReader parent w.aead in
   if authId i then
     let log : ideal_log w.region i = w.log in
@@ -220,7 +218,7 @@ val encrypt: #i:id -> e:writer i -> ad:adata i
   -> p:plain i ad r
   -> ST (cipher i)
        (requires (fun h0 ->
-         HyperHeap.disjoint e.region (AEAD.log_region e.aead) /\
+         disjoint e.region (AEAD.log_region e.aead) /\
          m_sel h0 (ctr e.counter) < max_ctr (alg i)))
        (ensures  (fun h0 c h1 ->
         modifies (Set.as_set [e.log_region; AEAD.log_region e.aead]) h0 h1
@@ -281,7 +279,7 @@ val decrypt: #i:id -> d:reader i -> ad:adata i -> c:cipher i
     /\ (match res with
        | None -> modifies Set.empty h0 h1
        | _    -> modifies_one d.region h0 h1
-                /\ modifies_rref d.region (Set.singleton (Heap.addr_of (as_ref ctr_counter_as_hsref))) h0.h h1.h
+                /\ modifies_ref d.region (Set.singleton (Heap.addr_of (as_ref ctr_counter_as_hsref))) h0.h h1.h
 	        /\ m_sel h1 (ctr d.counter) === j + 1)))
 
 #set-options "--z3rlimit 100 --max_fuel 0 --initial_fuel 1 --initial_ifuel 0 --max_ifuel 1"
