src/tls/DataStream.fst
@@ -6,13 +6,11 @@ module DataStream
 
 //* now generalized to include signals; rename to Stream?
 
-open FStar.Heap
-open FStar.HyperHeap
-open FStar.HyperStack
 open FStar.Seq
 open Platform.Bytes
 open Platform.Error
 
+open Mem
 open TLSError
 open TLSConstants
 open TLSInfo
@@ -104,22 +102,22 @@ type stream (i:id) = s: list (delta i) { wellformed i s }
 
 noeq type state (i:id) =
   | State: #region:rid ->
-           log: option (rref region (stream i)) { Some? log <==> authId i } ->
-           ctr: rref region nat ->
+           log: option (r: ref (stream i) {frameOf r = region}) { Some? log <==> authId i } ->
+           ctr: ref nat {frameOf ctr = region} ->
            state i
 
 (*
  * AR: adding the is_eternal_region refinement to satify the precondition of new_region.
  *)
-val gen: r0:rid{is_eternal_region r0} -> i:id -> ML (state i * state i)
+val gen: r0:rid{is_eternal_region r0 /\ witnessed(region_contains_pred r0)} -> i:id -> HyperStack.All.ML (state i * state i)
 let gen r0 (i:id) =
   let r = new_region r0 in
   empty_is_well_formed i;
   let t = ralloc r [] in
-  let log = if authId i then Some (mrref_of t) else None in
+  let log = if authId i then Some t else None in
   let ctr = ralloc r 0 in
-  let enc = State #i #r log (mrref_of ctr) in
-  let dec = State #i #r log (mrref_of ctr) in
+  let enc = State #i #r log ( ctr) in
+  let dec = State #i #r log ( ctr) in
   enc, dec
 
 // -------------------------------------------------------------
